FastMultiplication/ShorVerification/Implementation/PhaseProduct/Math/Table_Generation/Generator/Defs.lean
@@ -5,17 +5,60 @@ open Operations
 namespace Table_Generation
 
 def generatedPoints (mode : ProductMode) (k : ℕ) : List Point :=
-  match mode, k with
-  | .PhaseProduct, _ => []
-  | .PhaseTripleProduct, _ => []
+  canonicalPoints mode k
 
 def generatePointsInOrder (mode : ProductMode) (k : ℕ) (hk : k ≥ 2) : List Point :=
   match hk with
   | _ => generatedPoints mode k
 
-def generate (mode : ProductMode) (k : ℕ) (hk : k ≥ 2) : Prog k :=
-  match mode, hk with
-  | .PhaseProduct, _ => []
-  | .PhaseTripleProduct, _ => []
+def targetFirst : Prog 4 :=
+  (1 +:= 3 << 0) ;;
+  (2 +:= 0 << 0) ;;
+  (1 +:= 2 << 0) ;;
+  (2 <<s= 1) ;;
+  (2 -:= 1 << 0)
+
+def targetAtTwo : Prog 4 :=
+  (2 <<s= 2) ;;
+  (2 +:= 0 << 0) ;;
+  (1 +:= 3 << 2) ;;
+  (2 -:= 1 << 1) ;;
+  (1 <<s= 2) ;;
+  (1 +:= 2 << 0)
+
+def targetAtHalf : Prog 4 :=
+  (1 <<s= 2) ;;
+  (1 +:= 3 << 0) ;;
+  (2 +:= 0 << 2) ;;
+  (1 -:= 2 << 1) ;;
+  (2 <<s= 2) ;;
+  (2 +:= 1 << 0)
+
+def targetAtFour : Prog 4 :=
+  (2 <<s= 4) ;;
+  (2 +:= 0 << 0) ;;
+  (1 +:= 3 << 4) ;;
+  (2 -:= 1 << 2) ;;
+  (1 <<s= 3) ;;
+  (1 +:= 2 << 0)
+
+def targetGenerate : Prog 4 :=
+  targetFirst ;;
+  [valid_ops.phaseProduct 0, valid_ops.phaseProduct 3,
+    valid_ops.phaseProduct 1, valid_ops.phaseProduct 2] ;;
+  apply_Op_inverse targetFirst ;;
+  targetAtTwo ;;
+  [valid_ops.phaseProduct 1, valid_ops.phaseProduct 2] ;;
+  apply_Op_inverse targetAtTwo ;;
+  targetAtHalf ;;
+  [valid_ops.phaseProduct 2, valid_ops.phaseProduct 1] ;;
+  apply_Op_inverse targetAtHalf ;;
+  targetAtFour ;;
+  [valid_ops.phaseProduct 1, valid_ops.phaseProduct 2]
+
+def generate : (mode : ProductMode) → (k : ℕ) → (hk : k ≥ 2) → Prog k
+  | .PhaseTripleProduct, 4, _ => targetGenerate
+  | mode, k, hk =>
+      genOpsWithProduct (by omega) (generatePointsInOrder mode k hk)
 
 end Table_Generation
